Some experimentation with

src/Language/PlutusIR/Semantics/TypeSafety/Progress.v
@@ -2,8 +2,8 @@ Require Import PlutusCert.Language.PlutusIR.
 Import NamedTerm.
 Require Import PlutusCert.Language.PlutusIR.Semantics.Static.
 Require Import PlutusCert.Language.PlutusIR.Semantics.Static.Implementations.Named.
-Require Import PlutusCert.Language.PlutusIR.Semantics.Dynamic.Bigstep.
-
+Require Import PlutusCert.Language.PlutusIR.Semantics.Dynamic.
+Require Import PlutusCert.Language.PlutusIR.Semantics.TypeSafety.Preservation.
 Require Import Coq.Lists.List.
 
 Definition P_has_type (ctx : Context) (t : Term) (T : Ty) :=
@@ -75,3 +75,98 @@ Theorem progress : forall (t : Term) (T : Ty),
     emptyContext |-+ t : T ->
     exists v, t ==> v.
 Proof. Abort.
+
+
+Module e.
+
+Definition P_has_type (ctx : Context) (t : Term) (T : Ty) :=
+  ctx = emptyContext ->
+  (exists v, t ==> v) \/
+  ~(exists v, t ==> v).
+
+Definition P_constructor_well_formed ctx c := ctx |-ok_c c.
+
+Definition P_bindings_well_formed_nonrec ctx bs := 
+  forall t T,
+    ctx |-oks_nr bs ->
+    (append (flatten (map binds bs)) ctx) |-+ t : T ->
+    (exists v, eval_bindings_nonrec (Let NonRec bs t) v) \/
+    ~(exists v, eval_bindings_nonrec (Let NonRec bs t) v).
+
+Definition P_bindings_well_formed_rec ctx bs := ctx |-oks_r bs.
+
+Definition P_binding_well_formed (ctx : Context) b :=
+  forall s x Tb tb,
+    b = TermBind s (VarDecl x Tb) tb ->
+    exists vb, tb ==> vb.
+
+Axiom skip : forall P, P.
+
+Theorem preservation : forall t v T,
+    emptyContext |-+ t : T ->
+    t ==> v ->
+    emptyContext |-+ v : T.
+Proof. Admitted.
+
+Theorem progress' : forall (t : Term) (T : Ty) ,
+  emptyContext |-+ t : T ->
+  P_has_type emptyContext t T.
+Proof.
+  apply has_type__ind with P_constructor_well_formed P_bindings_well_formed_nonrec P_bindings_well_formed_rec P_binding_well_formed.
+  - intros. unfold P_has_type. intros.
+    subst.
+    destruct (H1 _ _ H0 H2). 
+    + destruct H.
+      left.
+      exists x.
+      apply E_Let.
+      assumption.
+    + right.
+      intros Hcon.
+      apply H.
+      destruct Hcon.
+      exists x.
+      inversion H4.
+      subst.
+      assumption. 
+  - intros. unfold P_has_type.
+    apply skip.
+  - intros. unfold P_has_type. intros.
+    subst. left. inversion H.
+  - intros. unfold P_has_type. intros.
+    apply skip.
+  - intros. unfold P_has_type. intros.
+    subst.
+    left.
+    exists (LamAbs x T1 t).
+    apply E_LamAbs.
+  - (* T_Apply *)
+    intros. unfold P_has_type. intros.
+    subst.
+    assert (emptyContext = emptyContext) by reflexivity.
+    apply H0 in H3 as H4.
+    apply H2 in H3 as H5.
+    destruct H4; destruct H5.
+    + destruct H4. destruct H5.
+      eapply preservation in H4 as H6; eauto.
+      apply eval_to_value in H4 as H7.
+      inversion H6; subst; inversion H7; subst; try solve [inversion H8; subst].
+      * assert (forall x s t6 t6', value s -> substitute x s t6 t6' -> (exists v, t6' ==> v) \/ ~(exists v, t6' ==> v)). {
+          apply skip.
+        }
+        apply eval_to_value in H5 as H9.
+        assert (exists t', substitute x1 x0 t t'). {
+          apply skip.
+        }
+        destruct H10.
+        eapply H8 in H9 as H14; try solve [apply H10].
+        destruct H14.
+        -- destruct H11.
+           left.
+           exists x2.
+           eapply E_Apply.
+           ++ apply H4.
+           ++ apply H5.
+           ++ apply H10.
+           ++ apply H11.
+Abort.
